Compute message signature in footer
The signature is computed as a pair of BigInteger's, (r, s), which is then converted into
a byte sequence. The byte sequence is expected to be of a particular length, according
to the ECDSA parameter. If (r, s) does not generate a byte sequence of the expected
length, then the code instead converts (r, N-s) to a byte sequence, where N is the order
of the group. If this byte sequence isn't of the right length, either, then the code gives
up trying.

This is similar to what ESDK Java and ESDK JavaScript do. However, those implementations
never give up. Instead, if neither (r, s) nor (r, N-s) produces a byte sequence of the
right length, then the process computes a new signature (r, s) and repeats. Possibly forever.

Maybe the code should retry a few times and then give up?

src/extern/dotnet/EncryptionExtern.cs
@@ -16,6 +16,7 @@ using Org.BouncyCastle.Math.EC;
 using Org.BouncyCastle.OpenSsl;
 using Org.BouncyCastle.Security;
 using Org.BouncyCastle.Asn1.X9;
+using Org.BouncyCastle.Asn1;
 
 using byteseq = Dafny.Sequence<byte>;
 
@@ -205,13 +206,12 @@ namespace Signature {
             }
         }
 
-        public static STL.Option<_System.Tuple2<byteseq, byteseq>> Sign(ECDSAParams x, byteseq sk, byteseq msg) {
+        public static STL.Option<byteseq> Sign(ECDSAParams x, byteseq sk, byteseq msg) {
             try {
                 X9ECParameters p;
                 if (x.is_ECDSA__P384) {
                     p = ECNamedCurveTable.GetByName("secp384r1");
-                }
-                else {
+                } else {
                     p = ECNamedCurveTable.GetByName("secp256r1");
                 }
                 ECDomainParameters dp = new ECDomainParameters(p.Curve, p.G, p.N, p.H);
@@ -219,14 +219,27 @@ namespace Signature {
                 ECDsaSigner sign = new ECDsaSigner();
                 sign.Init(true, skp);
                 BigInteger[] sig = sign.GenerateSignature(msg.Elements);
-                byte[] r = sig[0].ToByteArray();
-                byte[] s = sig[1].ToByteArray();
-                return new STL.Option_Some<_System.Tuple2<byteseq, byteseq>>(new _System.Tuple2<byteseq, byteseq>(new byteseq(r), new byteseq(s)));
-            }
-            catch {
-                return new STL.Option_None<_System.Tuple2<byteseq, byteseq>>();
+                byte[] bytes = SignatureToByteArray(sig[0], sig[1]);
+                if (bytes.Length != x.SignatureLength()) {
+                    // Most of the time, a signature of the wrong length can be fixed
+                    // be negating s in the signature relative to the group order.
+                    bytes = SignatureToByteArray(sig[0], p.N.Subtract(sig[1]));
+                    if (bytes.Length != x.SignatureLength()) {
+                        // We give up. :(
+                        return new STL.Option_None<byteseq>();
+                    }
+                }
+                // Note, the postcondition of this method says that a Some? return must contain a
+                // sequence of bytes whose length is x.SignatureLength().
+                return new STL.Option_Some<byteseq>(new byteseq(bytes));
+            } catch {
+                return new STL.Option_None<byteseq>();
             }
         }
 
+        private static byte[] SignatureToByteArray(BigInteger r, BigInteger s) {
+            DerSequence derSeq = new DerSequence(new DerInteger(r), new DerInteger(s));
+            return derSeq.GetEncoded();
+        }
     }
 }
